Revise semantic typing for primitives, reorder rules
(Adds compile error due to missing import).

theories/Dot/lr/lr_lemmasPrim.v
@@ -1,14 +1,24 @@
 From iris.proofmode Require Import tactics.
-From D.Dot Require Import unary_lr.
+From D.Dot Require Import syn prim_typing.
 From D.pure_program_logic Require Import lifting.
 From iris.program_logic Require Import language.
 
 From D.Dot Require Import rules unary_lr.
 
-Implicit Types (L T U: ty) (v: vl) (e: tm) (d: dm) (ds: dms) (Γ : ctx).
+Implicit Types (v: vl) (e: tm) (d: dm) (ds: dms) (n : nat).
+
+Inductive cond_bin_op_syntype : bin_op → ∀ (B1 B2 Br : base_ty),
+  (prim_sem B1 → prim_sem B2 → Prop) → Set :=
+| ty_syn b B1 B2 Br : bin_op_syntype b B1 B2 Br →
+                      cond_bin_op_syntype b B1 B2 Br (const (const True))
+| ty_bminus         : cond_bin_op_syntype bminus tnat  tnat  tnat  (λ n1 n2, n2 ≤ n1)
+| ty_bdiv           : cond_bin_op_syntype bdiv   tnat  tnat  tnat  (λ _ n, n > 0).
 
 Definition un_op_semtype u B1 Br := ∀ v, pure_interp_prim B1 v →
   ∃ w, un_op_eval u v = Some w ∧ pure_interp_prim Br w.
+
+Lemma un_op_syntype_sound {u B1 Br} : un_op_syntype u B1 Br → un_op_semtype u B1 Br.
+Proof. rewrite /un_op_semtype /pure_interp_prim => Ht; inverse Ht; naive_solver. Qed.
 
 Definition bin_op_semtype b B1 B2 Br (P : prim_sem B1 → prim_sem B2 → Prop) :=
   ∀ v1 v2 l1 l2,
@@ -17,41 +27,29 @@ Definition bin_op_semtype b B1 B2 Br (P : prim_sem B1 → prim_sem B2 → Prop) 
   P l1 l2 →
   ∃ w, bin_op_eval b v1 v2 = Some w ∧ pure_interp_prim Br w.
 
-Inductive un_op_syntype : un_op → base_ty → base_ty → Set :=
-| ty_unot : un_op_syntype unot tbool tbool.
+Lemma bin_op_syntype_sound {b B1 B2 Br} :
+  bin_op_syntype b B1 B2 Br → bin_op_semtype b B1 B2 Br (const (const True)).
+Proof. rewrite /bin_op_semtype /pure_interp_prim. destruct 1; naive_solver. Qed.
 
-Inductive bin_op_syntype : bin_op → ∀ (B1 B2 Br : base_ty),
-  (prim_sem B1 → prim_sem B2 → Prop) → Set :=
-| ty_beq_bool : bin_op_syntype beq    tbool tbool tbool (const (const True))
-| ty_beq_nat  : bin_op_syntype beq    tnat  tnat  tbool (const (const True))
-| ty_blt      : bin_op_syntype blt    tnat  tnat  tbool (const (const True))
-| ty_ble      : bin_op_syntype ble    tnat  tnat  tbool (const (const True))
-| ty_bplus    : bin_op_syntype bplus  tnat  tnat  tnat  (const (const True))
-| ty_bminus   : bin_op_syntype bminus tnat  tnat  tnat  (λ n1 n2, n2 ≤ n1)
-| ty_btimes   : bin_op_syntype btimes tnat  tnat  tnat  (const (const True))
-| ty_bdiv     : bin_op_syntype bdiv   tnat  tnat  tnat  (λ _ n, n > 0).
-
-Lemma un_op_syntype_sound {u B1 Br} : un_op_syntype u B1 Br → un_op_semtype u B1 Br.
-Proof. rewrite /un_op_semtype /pure_interp_prim => Ht; inverse Ht; naive_solver. Qed.
-
-Lemma bin_op_syntype_sound {b B1 B2 Br P} :
-  bin_op_syntype b B1 B2 Br P → bin_op_semtype b B1 B2 Br P.
+Lemma cond_bin_op_syntype_sound {b B1 B2 Br P} :
+  cond_bin_op_syntype b B1 B2 Br P → bin_op_semtype b B1 B2 Br P.
 Proof.
-  rewrite /bin_op_semtype /pure_interp_prim => Ht;
-    dependent destruction Ht => *; simplify_eq/=;
-    try (case_decide || case_match);
-    naive_solver eauto with lia.
+  destruct 1; first exact: bin_op_syntype_sound;
+    rewrite /bin_op_semtype /pure_interp_prim => *; simplify_eq/=;
+    try (case_decide || case_match); naive_solver eauto with lia.
 Qed.
 
 Section Sec.
-  Context `{HdlangG: dlangG Σ} Γ.
+  Context `{HdlangG: dlangG Σ}.
 
-  Lemma T_Nat_I n: Γ ⊨ tv (vnat n): TNat.
+  Lemma sT_Nat_I Γ n: Γ s⊨ tv (vnat n): oNat.
   Proof. iIntros "!> * _ /="; rewrite -wp_value /= /pure_interp_prim /prim_evals_to; eauto. Qed.
 
-  Lemma T_Bool_I b: Γ ⊨ tv (vlit $ lbool b): TPrim tbool.
+  Lemma sT_Bool_I Γ b: Γ s⊨ tv (vbool b): oBool.
   Proof. iIntros "!> * _ /="; rewrite -wp_value /= /pure_interp_prim /prim_evals_to; eauto. Qed.
 
+
+  (** * Unary operations *)
   Lemma wp_un B1 Br u v
     (Hev1 : pure_interp_prim B1 v) (Hu : un_op_semtype u B1 Br) :
     WP tun u (tv v) {{ w, ⌜un_op_eval u v = Some w ∧ pure_interp_prim Br w⌝ }}%I.
@@ -60,9 +58,9 @@ Section Sec.
     by rewrite -wp_pure_step_later // -wp_value'; auto.
   Qed.
 
-  Lemma T_Un u e1 B1 Br (Hu : un_op_semtype u B1 Br) :
-    Γ ⊨ e1 : TPrim B1 -∗
-    Γ ⊨ tun u e1 : TPrim Br.
+  Lemma sT_Un Γ u e1 B1 Br (Hu : un_op_semtype u B1 Br) :
+    Γ s⊨ e1 : oPrim B1 -∗
+    Γ s⊨ tun u e1 : oPrim Br.
   Proof.
     iIntros "#He1 !>" (ρ) "#Hg !>".
     smart_wp_bind (UnCtx _) v1 "#Ha1" ("He1" with "Hg"); iClear "He1 Hg".
@@ -70,6 +68,12 @@ Section Sec.
     by iApply wp_wand; [iApply wp_un|iIntros (? [??])].
   Qed.
 
+  Lemma T_Un Γ u e1 B1 Br (Hu : un_op_syntype u B1 Br) :
+    Γ ⊨ e1 : TPrim B1 -∗
+    Γ ⊨ tun u e1 : TPrim Br.
+  Proof. apply sT_Un, un_op_syntype_sound, Hu. Qed.
+
+  (** * Binary operations *)
   Lemma wp_bin {b v1 v2 B1 B2 Br P} (Hu : bin_op_semtype b B1 B2 Br P) l1 l2
     (Hev1 : prim_evals_to B1 v1 l1) (Hev2 : prim_evals_to B2 v2 l2)
     (HP : P l1 l2) :
@@ -79,10 +83,10 @@ Section Sec.
     by rewrite -wp_pure_step_later // -wp_value'; auto.
   Qed.
 
-  Lemma T_Bin b e1 e2 B1 B2 Br (Hu : bin_op_semtype b B1 B2 Br (const (const True))) :
-    Γ ⊨ e1 : TPrim B1 -∗
-    Γ ⊨ e2 : TPrim B2 -∗
-    Γ ⊨ tbin b e1 e2 : TPrim Br.
+  Lemma sT_Bin Γ b e1 e2 B1 B2 Br (Hu : bin_op_semtype b B1 B2 Br (const (const True))) :
+    Γ s⊨ e1 : oPrim B1 -∗
+    Γ s⊨ e2 : oPrim B2 -∗
+    Γ s⊨ tbin b e1 e2 : oPrim Br.
   Proof.
     iIntros "#He1 #He2 !> /=" (ρ) "#Hg !>". rewrite /oPrim/= /pure_interp_prim.
     smart_wp_bind (BinLCtx _ _) v1 "#Ha1" ("He1" with "Hg"); iClear "He1".
@@ -92,26 +96,26 @@ Section Sec.
     by iApply wp_wand; [iApply wp_bin|iIntros (? [??])].
   Qed.
 
-  Lemma T_Un' u e1 B1 Br (Hu : un_op_syntype u B1 Br) :
-    Γ ⊨ e1 : TPrim B1 -∗
-    Γ ⊨ tun u e1 : TPrim Br.
-  Proof. apply T_Un, un_op_syntype_sound, Hu. Qed.
+  Lemma sT_Bin_cond Γ b e1 e2 B1 B2 Br (Hu : cond_bin_op_syntype b B1 B2 Br (const (const True))) :
+    Γ s⊨ e1 : oPrim B1 -∗
+    Γ s⊨ e2 : oPrim B2 -∗
+    Γ s⊨ tbin b e1 e2 : oPrim Br.
+  Proof. apply sT_Bin, cond_bin_op_syntype_sound, Hu. Qed.
 
-  Lemma T_Bin' b e1 e2 B1 B2 Br (Hu : bin_op_syntype b B1 B2 Br (const (const True))) :
+  Lemma T_Bin Γ b e1 e2 B1 B2 Br (Hu : bin_op_syntype b B1 B2 Br) :
     Γ ⊨ e1 : TPrim B1 -∗
     Γ ⊨ e2 : TPrim B2 -∗
     Γ ⊨ tbin b e1 e2 : TPrim Br.
-  Proof. apply T_Bin, bin_op_syntype_sound, Hu. Qed.
+  Proof. apply sT_Bin_cond, ty_syn, Hu. Qed.
 
-  Lemma T_If e e1 e2 T :
-    Γ ⊨ e : TBool -∗
-    Γ ⊨ e1 : T -∗
-    Γ ⊨ e2 : T -∗
-    Γ ⊨ tif e e1 e2 : T.
+  Lemma sT_If Γ e e1 e2 T :
+    Γ s⊨ e : oBool -∗ Γ s⊨ e1 : T -∗ Γ s⊨ e2 : T -∗
+    Γ s⊨ tif e e1 e2 : T.
   Proof.
     iIntros "#He #He1 #He2 !> /=" (ρ) "#Hg !>".
     smart_wp_bind (IfCtx _ _) v "#Ha" ("He" with "[]").
-    iDestruct "Ha" as %([] & ->); rewrite -wp_pure_step_later //;
+    rewrite /pure_interp_prim/=; iDestruct "Ha" as %([] & ->);
+      (rewrite -wp_pure_step_later; last done);
       [ iApply ("He1" with "Hg") | iApply ("He2" with "Hg")].
   Qed.
 End Sec.
